> A pole of negligible mass leans against a wall, at angle $\theta$ with the horizontal. Gravity is directed down.
> **(a)** Find the constraint relating the vertical acceleration of one end to the horizontal acceleration of the other.
 > **(b)** Now suppose that each end carries a pivoted mass $M$. Find the initial vertical and horizontal components of acceleration as the pole just begins to slide on the frictionless wall and floor. Assume that at the beginning of the motion the forces exerted by the rod are along the line of the rod. (As the motion progresses, the system rotates and the rod exerts sidewise forces.)
 > ![[Pasted image 20240319142511.png]]
 
# (a)
 
 Sendo $a$ a posi√ß√£o horizontal da ponta inicialmente mais baixa
$$b^2 + a^2 = L^2$$
 $L$ √© constante. Derivando ambos os lados em fun√ß√£o do tempo para obter as velocidades. $a$ e $b$ s√£o fun√ß√µes de $t$, portanto aplica-se a [[regra da cadeia]] 
$$\begin{align}
\frac{d}{dt} b(t)^2 + \frac{d}{dt} a(t)^2 &= \frac{d}{dt} L^2 \\
2b \frac{d}{dt} b + 2a\frac{d}{dt} a &= 0 \\
2(b\dot{b} + a\dot{a}) &= 0 \\
b\dot{b} + a\dot{a} &= 0
\end{align}$$
Derivando novamente para obter a acelera√ß√£o,
$$\begin{align}
\frac{d}{dt}(b\dot{b}) + \frac{d}{dt}(a\dot{a}) &= 0 \\
(\dot{b}\dot{b}+b\ddot{b}) + (\dot{a}\dot{a} + a\ddot{a}) &= 0 \\
\dot{b}^2 + b\ddot{b} + \dot{a}^2 + a\ddot{a} &= 0
\end{align}$$
# (b)
J√° que a vara est√° come√ßando a escorregar, temos velocidade inicial nula ($\dot{a} = 0$, $\dot{b} = 0$). Assim, a restri√ß√£o encontrada em [[#(a)]] se torna
$$\begin{align}
b\ddot{b} + a\ddot{a} &= 0 \\
a\ddot{a} &= -b\ddot{b} \\
\frac{\ddot{a}}{\ddot{b}} &= -\frac{b}{a} = -\tan\theta
\end{align}$$
![[2.7 Leaning pole 2024-03-19 16.56.35.excalidraw|500]]
%%[[2.7 Leaning pole 2024-03-19 16.56.35.excalidraw.md|üñã Edit in Excalidraw]]%%
$$\begin{rcases}
M_{b}\ddot{b} = F_{p}\sin\theta - M_{b}g \\
M_{a}\ddot{a} = F_{p}\cos\theta
\end{rcases} \implies
\frac{M_{b}}{\sin\theta}(\ddot{b}+g) = \frac{M_{a}}{\cos\theta}\ddot{a}$$
$$\begin{align}
M_{b}(\ddot{b}+g) &= M_{a}\ddot{a}\cancelto{\tan\theta}{\frac{\sin\theta}{\cos\theta}}
\end{align}$$
No caso do exerc√≠cio $M_{a} = M_{b}$, portanto
$$\ddot{b}+g = \ddot{a} \tan\theta$$
Resolvendo para $\ddot{b}$, substitu√≠mos $\ddot{a} = -\ddot{b}\tan\theta$
$$\begin{align}
\ddot{b} = -\ddot{b}\tan^2\theta - g \\
\ddot{b}(1+\tan^2\theta) = -g \\
\ddot{b} = -g\frac{1}{1+\tan^2\theta}
\end{align}$$
Resolvendo para $\ddot{a}$, substitu√≠mos $\ddot{b} = -\ddot{a}/\tan\theta$:
$$\begin{align}
\ddot{a}\tan\theta &= g - \frac{\ddot{a}}{\tan\theta} \\
\ddot{a}\tan^2\theta &= g\tan\theta - \ddot{a} \\
\ddot{a}(1+\tan^2\theta) &= g\tan\theta \\
\ddot{a} &= g\tan\theta\frac{1}{1+\tan\theta}
\end{align}$$
Podemos provar que $1/(1+\tan^2\theta) = \cos^2\theta$ usando as identidades $\tan\theta = \sin\theta/\cos\theta$ e $\cos^2\theta + \sin^2\theta = 1$:
$$\frac{1}{1+\tan^2\theta} = \frac{\cos^2\theta}{\cancelto{1}{\cos^2\theta + \cancel{\cos^2\theta} \frac{\sin^2\theta}{\cancel{\cos^2\theta}}}} = \cos^2\theta$$
Assim, finalmente temos
$$\begin{cases}
\ddot{a} &= g\tan\theta \cos^2\theta = g\frac{\sin\theta}{\cancel{\cos\theta}}\cos^\cancel{2}\theta  = g\sin\theta \cos\theta\\
\ddot{b} &= -g\cos^2\theta
\end{cases}$$