> This problem involves solving a simple diÔ¨Äerential equation.
> A block of mass $m$ slides on a frictionless table. It is constrained to move inside a ring of radius $l$ that is fixed to the table. At $t = 0$, the block is moving along the inside of the ring (in the tangential direction) with velocity $v_{0}$. The coeÔ¨Écient of friction between the block and the ring is $\mu$.
>**(a)** Find the velocity of the block at later times.
>**(b)** Find the position of the block at later times.
>![[Pasted image 20240414223930.png]]

![[3.23 Mass and ring* 2024-04-14 22.46.31.excalidraw]]
%%[[3.23 Mass and ring* 2024-04-14 22.46.31.excalidraw.md|üñã Edit in Excalidraw]]%%
$ml\omega^2 - N = 0 \implies N = ml\omega^2$
$F = \mu N = \mu ml\omega^2$
$a = F/m = (\mu \cancel{m}l\omega^2)/\cancel{m} = -\mu l(v/l)^2 = -\mu v^2/l$

# (a)
$$\begin{align}
\frac{dv}{dt} &= -\frac{\mu v^2}{l} \\
\frac{dv}{v^2} &= -\frac{\mu}{l} dt \\
\int \frac{1}{v^2} \, dv &= -\frac{\mu}{l} \int  \, dt \\
-\frac{1}{v} + \frac{1}{v_{0}} &= -\frac{\mu t}{l} \\
\frac{1}{v} &= \frac{1}{v_{0}} + \frac{\mu t}{l} \\
v &= \left( \frac{1}{v_{0}} + \frac{\mu t}{l} \right)^{-1}
\end{align}$$

# (b)
Sendo um movimento circular peri√≥dico, n√≥s queremos a posi√ß√£o angular $\theta$, onde $\dot{\theta} = v/l$
$$\begin{align}
\dot{\theta} &= \left( l \left( \frac{1}{v_{0}} + \frac{\mu t}{l} \right) \right)^{-1} \\
\int \frac{d\theta}{dt} \, dt &= \int \left( \frac{l}{v_{0}} + \mu t \right)^{-1} \, dt
\end{align}$$
Definamos $u = l/v_{0} + \mu t$
$$\begin{align}
u &= \frac{l}{v_{0}} + \mu t  \\
\frac{du}{dt} &= \cancel{\frac{d}{dt} \frac{l}{v_{0}}} + \frac{d}{dt} \mu t  \\
du &= \mu \, dt \\
dt &= \frac{du}{\mu}
\end{align}$$
Substituindo, temos
$$\int  \, d\theta  = \frac{1}{\mu} \int \frac{1}{u} \, du$$
Queremos integrar de $t=0$ a um valor qualquer de $t$. Definindo $\theta_{0}$ como a posi√ß√£o angular em $t=0$,
$$\begin{align}
\theta - \theta_{0} &= \frac{1}{\mu} [\ln u(t) - \ln u(0)] \\
\theta &= \theta_{0} + \frac{1}{\mu} \left[ \ln\left( \frac{l}{v_{0}} + \mu t \right) - \ln\left( \frac{l}{v_{0}} + \cancel{\mu 0} \right) \right] \\
\theta &= \theta_{0} + \frac{1}{\mu} \ln\left( \frac{\frac{l}{v_{0}} + \mu t}{\frac{l}{v_{0}}} \right) \\
\theta &= \theta_{0} + \frac{1}{\mu} \ln\left( 1 + \mu t \frac{v_{0}}{l} \right) \\
\theta &= \theta_{0} + \frac{1}{\mu} \ln\left( 1 + \mu t \frac{v_{0}}{l} \right)
\end{align}$$
(Do segundo para o terceiro passo, aplica-se a [[Identidades Not√°veis#Diferen√ßa de logaritmos]])