> This problem involves a simple diﬀerential equation. You should be able to integrate it after a little “playing around.”
> A particle of mass $m$ moving along a straight line is acted on by a retarding force (one always directed against the motion) $F = be^{av}$, where $b$ and $a$ are constants and $v$ is the velocity. At $t=0$ it is moving with velocity $v_{0}$ . Find the velocity at later times.





$$\begin{align}
m \frac{dv}{dt} &= -F \\
m \frac{dv}{dt} &= -be^{av} \\
e^{-av} dv &= -\frac{b}{m} dt \\
\int e^{-av} \, dv  &= - \int \frac{b}{m} \, dt \\
\int_{v_{0}}^{v_{1}} e^{-av} \, dv  &= -\frac{b}{m} \int_{0}^{t_{1}} \, dt
\end{align}$$
Definindo $u = -av$:
$$\frac{du}{dt} = \frac{d}{dt} (-av) \implies
\frac{du}{dt} = -a\frac{dv}{dt} \implies
\frac{du}{-a} = dv$$
Substituindo então,
$$\begin{align}
\int_{v_{0}}^{v_{1}} \frac{e^{u}}{-a} \, du  &= -\frac{b}{m} \int_{0}^{t_{1}} \, dt \\
\frac{1}{-a}(e^{-av_{1}} - e^{-av_{0}}) &= -\frac{bt_{1}}{m} \\
e^{-av_{1}} - e^{-av_{0}} &= \frac{abt_{1}}{m} \\
e^{-av_{1}} &= e^{-av_{0}} + \frac{abt_{1}}{m} \\
-av_{1} &= \ln\left( e^{-av_{0}} + \frac{abt_{1}}{m} \right) \\
v_{1} &= -\frac{1}{a}\ln\left( e^{-av_{0}} + \frac{abt_{1}}{m} \right) \\
v_{1} &= \frac{1}{a}\ln\left( \frac{1}{e^{-av_{0}} + \frac{abt_{1}}{m}} \right)
\end{align}$$
